LeanSubst/Types/Nat.lean
@@ -11,7 +11,7 @@ def Nat.rmap (r : Ren T) : Nat -> Nat
 | n => r.act n
 
 instance : RenMap Nat [T] where
-  rmap r := Nat.rmap r.1
+  rmap r := Nat.rmap r.head
 
 theorem Nat.rmap_simp {r : Ren T} {n : Nat} : n⟨r⟩ = r.act n := by simp [RenMap.rmap, Nat.rmap]
 
